Linglib.lean
@@ -108,10 +108,10 @@ import Linglib.Core.Computability.Variety.Langs
 import Linglib.Core.Data.Fin.Tuple.Basic
 import Linglib.Core.Data.Fintype.Sets
 import Linglib.Core.Data.Fintype.Transfer
-import Linglib.Core.Data.List.Agree
 import Linglib.Core.Data.List.Bookend
 import Linglib.Core.Data.List.Chain
 import Linglib.Core.Data.List.Destutter
+import Linglib.Core.Data.List.EqOn
 import Linglib.Core.Data.List.DropRight
 import Linglib.Core.Data.List.Factors
 import Linglib.Core.Data.List.Fold
